\begin{prooftree}
    \AxiomC{$E \equiv E_1[E_2]$}
    \UnaryInfC{$[E_1] \neq object(),$} \noLine
    \UnaryInfC{$if ([E_1] = string()) => [E] = string(),$} \noLine
    \UnaryInfC{$if ([E_1] = array(\{types\})) => [E] <: \{types\},$} \noLine
    \UnaryInfC{$if ([E_1] \neq string() \land [E_1] \neq array(\_)) => [E] = null()$}
\end{prooftree} 

% previous values
%\begin{prooftree}
%    \AxiomC{$E_1[E_2]$ $\land$ $[E_1] == string()$}
%    \UnaryInfC{$[E_1[E_2]] = string()$}
%\end{prooftree} 
%\begin{prooftree}
%    \AxiomC{$E_1[E_2]$ $\land$ $[E_1] == array()$}
%    \UnaryInfC{$[E_1[E_2]] <: any()$}
%\end{prooftree} 
%\begin{prooftree}
%    \AxiomC{$E_1[E_2]$ $\land$ $(E_1 == string()$ $\lor$ [$E_1] == array())$}
%    \UnaryInfC{$[E_1[E_2]] = null()$}
%\end{prooftree} 
