\begin{prooftree}
    \AxiomC{$E \equiv (E_1 + E_2)$}
    \UnaryInfC{$[E] <: array(\_) \lor [E] <: float(),$} \noLine
    \UnaryInfC{$if([E_1] <: array(\_) \land [E_2] <: array(\_)) => [E] <: array(\_),$} \noLine
    \UnaryInfC{$if([E_1] !<: array(\_) \lor [E_2] !<: array(\_)) => [E] <: float()$}
\end{prooftree}
\begin{prooftree}
    \AxiomC{$E \equiv (E_1 - E_2) \lor (E_1 * E_2) \lor (E_1 / E_2)$}
    \UnaryInfC{$[E] <: float(),$} \noLine
    \UnaryInfC{$[E_1] \neq array(\_),$} \noLine
    \UnaryInfC{$[E_2] \neq array(\_)$}
\end{prooftree}
\begin{prooftree}
    \AxiomC{$E \equiv (E_1 \; \% \; E_2) \lor (E_1 << E_2) \lor (E_1 >> E_2)$}
    \UnaryInfC{$[E] = integer()$}
\end{prooftree}
\begin{prooftree}
    \AxiomC{$E \equiv (E_1 \; \& \; E_2) \lor (E_1 \; \vert \; E_2) \lor (E_1 \; $\^{}$ \; E_2)$}
    \UnaryInfC{$[E] = string() \lor [E] = integer(),$} \noLine
    \UnaryInfC{$if([E_1] = string() \land [E_2] = string()) => [E] = string(),$} \noLine
    \UnaryInfC{$if([E_1] \neq string() \lor [E_2] \neq string()) => [E] = integer()$}
\end{prooftree}
