\begin{center}
\begin{bprooftree}
    \AxiomC{$E \equiv $ ($E_1$ $==$ $E_2$)}
    \UnaryInfC{$\llbracket{}E\rrbracket{} = booleanType()$}
\end{bprooftree}   
\begin{bprooftree}
    \AxiomC{$E \equiv $ ($E_1$ $===$ $E_2$)}
    \UnaryInfC{$\llbracket{}E\rrbracket{} = booleanType()$}
\end{bprooftree}   
\begin{bprooftree}
    \AxiomC{$E \equiv $ ($E_1$ $!=$ $E_2$)}
    \UnaryInfC{$\llbracket{}E\rrbracket{} = booleanType()$}
\end{bprooftree}   
\\
\vspace{1em}
\begin{bprooftree}
    \AxiomC{$E \equiv $ ($E_1$ $<>$ $E_2$)} 
    \UnaryInfC{$\llbracket{}E\rrbracket{} = booleanType()$}
\end{bprooftree}   
\begin{bprooftree}
    \AxiomC{$E \equiv $ ($E_1$ $!==$ $E_2$)}
    \UnaryInfC{$\llbracket{}E\rrbracket{} = booleanType()$}
\end{bprooftree}   
\begin{bprooftree}
    \AxiomC{$E \equiv $ ($E_1$ $<$ $E_2$)}
    \UnaryInfC{$\llbracket{}E\rrbracket{} = booleanType()$}
\end{bprooftree}   
\\
\vspace{1em}
\begin{bprooftree}
    \AxiomC{$E \equiv $ ($E_1$ $>$ $E_2$)}
    \UnaryInfC{$\llbracket{}E\rrbracket{} = booleanType()$}
\end{bprooftree}   
\begin{bprooftree}
    \AxiomC{$E \equiv $ ($E_1$ $<=$ $E_2$)}
    \UnaryInfC{$\llbracket{}E\rrbracket{} = booleanType()$}
\end{bprooftree}   
\begin{bprooftree}
    \AxiomC{$E \equiv $ ($E_1$ $>=$ $E_2$)}
    \UnaryInfC{$\llbracket{}E\rrbracket{} = booleanType()$}
\end{bprooftree}   
\end{center}   
