\begin{center}
\begin{bprooftree}
    \AxiomC{$E \equiv $ ($E_1$ $and$ $E_2$)}
    \RightLabel{(i)}
    \UnaryInfC{$[E] = boolean()$}
\end{bprooftree}   
\begin{bprooftree}
    \AxiomC{$E \equiv $ ($E_1$ $or$ $E_2$)}
    \RightLabel{(ii)}
    \UnaryInfC{$[E] = boolean()$}
\end{bprooftree}   
\begin{bprooftree}
    \AxiomC{$E \equiv $ ($E_1$ $xor$ $E_2$)}
    \RightLabel{(iii)}
    \UnaryInfC{$[E] = boolean()$}
\end{bprooftree}   
\\
\vspace{1em}
\begin{bprooftree}
    \AxiomC{$E \equiv $ ($E_1$ $\&\&$ $E_2$)}
    \RightLabel{(iv)}
    \UnaryInfC{$[E] = boolean()$}
\end{bprooftree}   
\begin{bprooftree}
    \AxiomC{$E \equiv $ ($E_1$ $\vert\vert$ $E_2$)}
    \RightLabel{(v)}
    \UnaryInfC{$[E] = boolean()$}
\end{bprooftree}   
\end{center}   
